{
 "cells": [
  {
   "cell_type": "markdown",
   "metadata": {},
   "source": [
    "## Cut rule\n",
    "The cut rule allows us to combine statements if an expression appears on the hyptothesis of one statement, and the conclusion of another.\n",
    "\n",
    "Here is an example:\n",
    "$$\n",
    "\\frac\n",
    "{F \\rightarrow A, B \\quad F', A \\rightarrow B'}\n",
    "{F, F' \\rightarrow B, B'}\n",
    "$$"
   ]
  },
  {
   "cell_type": "markdown",
   "metadata": {},
   "source": [
    "## More rules\n",
    "\n",
    "Here are some more logic rules\n",
    "\n",
    "$$\n",
    "\\frac{A \\vdash X \\quad A \\vdash Y}{A \\vdash X \\land Y} \\quad (\\land)\n",
    "$$\n",
    "\n",
    "$$\n",
    "\\frac{A, X \\vdash Z \\quad A, Y \\vdash Z}{A, X \\lor Y \\vdash Z} \\quad (\\lor)\n",
    "$$\n",
    "\n",
    "$$\n",
    "\\frac{A \\vdash X \\quad A \\vdash Y}{A \\vdash X \\rightarrow Y} \\quad (\\rightarrow)\n",
    "$$\n",
    "\n",
    "These rules should have a double line since they work in both ways, going down __introduces the connective__ and going up __eliminates the connective__.\n",
    "\n",
    "For example if from A we can derive X and from A we can derive Y (as in the first rule), then it follows that we derive X and Y from A. Likewise if we can derived X and Y from A, then we can derive X from A and Y from A. "
   ]
  },
  {
   "cell_type": "markdown",
   "metadata": {},
   "source": [
    "## Example proof\n",
    "\n",
    "$$\n",
    "\\overline{A \\rightarrow (B \\rightarrow C) \\vdash A \\rightarrow (B \\rightarrow C)}^{\\quad\\displaystyle(I)}\n",
    "\\\\\n",
    "\\overline{A \\rightarrow (B \\rightarrow C), A \\vdash B \\rightarrow C}^{\\quad\\displaystyle(\\rightarrow^-)}\n",
    "\\\\\n",
    "\\overline{A \\rightarrow (B \\rightarrow C), B, A \\vdash C}^{\\quad\\displaystyle(\\rightarrow^-)}\n",
    "\\\\\n",
    "\\overline{A \\rightarrow (B \\rightarrow C), B \\vdash (A \\rightarrow C)}^{\\quad\\displaystyle(\\rightarrow^+)}\n",
    "\\\\\n",
    "\\overline{A \\rightarrow (B \\rightarrow C) \\vdash B \\rightarrow (A \\rightarrow C)}^{\\quad\\displaystyle(\\rightarrow^+)}\n",
    "$$"
   ]
  },
  {
   "cell_type": "markdown",
   "metadata": {},
   "source": [
    "## Another proof\n",
    "\n",
    "$$\n",
    "\\dfrac\n",
    "{\n",
    "\\dfrac{\\overline{A \\lor B \\vdash A \\lor B}}{A \\lor B \\vdash A} \n",
    "\\quad \n",
    "\\dfrac{\\overline{A \\lor B \\vdash A \\lor B}}{A \\vdash A \\lor B}\n",
    "}\n",
    "{A \\lor B \\vdash A \\land B}\n",
    "$$\n",
    "\n",
    "The problem here is that for the cut, we could have choosen B. For more complicated proofs their can be many diffrent possibilitys but only one that works."
   ]
  },
  {
   "cell_type": "markdown",
   "metadata": {},
   "source": [
    "## Gentzen's Rules\n",
    "\n",
    "A sequent, $A \\vdash B$ is valid iff\n",
    "- every expression in $A$ is true\n",
    "- some expression in $B$ is true\n",
    "\n",
    "$$\n",
    "\\overline{\\Gamma, A \\vdash \\Delta, A}^{\\quad\\displaystyle(I)}\n",
    "$$\n",
    "\n",
    "$$\n",
    "\\frac{\\Gamma, A, B \\vdash \\Delta}{\\Gamma, A \\land B \\vdash \\Delta}\n",
    "\\quad (\\land L)\n",
    "$$\n",
    "\n",
    "$$\n",
    "\\frac{\\Gamma, A \\vdash \\Delta \\quad \\Gamma, B \\vdash \\Delta}{\\Gamma, A \\lor B \\vdash \\Delta}\n",
    "\\quad (\\lor L)\n",
    "$$\n",
    "\n",
    "$$\n",
    "\\frac{\\Gamma \\vdash A, B, \\Delta}{\\Gamma \\vdash A \\land B, \\Delta}\n",
    "\\quad (\\lor R)\n",
    "$$\n",
    "\n",
    "$$\n",
    "\\frac{\\Gamma \\vdash A, \\Delta \\quad \\Gamma \\vdash B, \\Delta}{\\Gamma \\vdash A \\land B, \\Delta}\n",
    "\\quad (\\land R)\n",
    "$$\n",
    "\n",
    "$$\n",
    "\\frac{\\Gamma \\vdash A, \\Delta \\quad \\Gamma \\vdash B, \\Delta}{\\Gamma, A \\rightarrow B \\vdash \\Delta}\n",
    "\\quad (\\rightarrow L)\n",
    "$$\n",
    "\n",
    "$$\n",
    "\\frac{\\Gamma, A \\vdash B, \\Delta}{\\Gamma \\vdash A \\rightarrow B, \\Delta}\n",
    "\\quad (\\rightarrow R)\n",
    "$$\n",
    "\n",
    "$$\n",
    "\\frac{\\Gamma \\vdash A,\\Delta}{\\Gamma, ¬A \\vdash \\Delta}\n",
    "\\quad (¬L)\n",
    "$$\n",
    "\n",
    "$$\n",
    "\\frac{\\Gamma, A \\vdash \\Delta}{\\Gamma \\vdash ¬A, \\Delta}\n",
    "\\quad (¬R)\n",
    "$$"
   ]
  },
  {
   "cell_type": "markdown",
   "metadata": {},
   "source": [
    "Going back to the previous proof, we can now remove the need for a cut by using the rules above\n",
    "\n",
    "$$\n",
    "\\overline{A, B \\vdash A, B}^{\\quad\\displaystyle(I)} \\\\\n",
    "\\overline{A \\land B \\vdash A , B}^{\\quad\\displaystyle(\\land L)} \\\\\n",
    "\\overline{A \\land B \\vdash A \\lor B}^{\\quad\\displaystyle(\\lor R)}\\\\\n",
    "$$"
   ]
  },
  {
   "cell_type": "markdown",
   "metadata": {},
   "source": [
    "Lets look at a more complex proof, say we want to prove:\n",
    "$$\n",
    "A \\rightarrow (B \\rightarrow C) \\vdash B \\rightarrow (A \\rightarrow C)\n",
    "$$\n",
    "\n",
    "First we find the a conclusion of one of the rules that matches the pattern of the expression which is in this case is $(\\rightarrow R)$\n",
    "\n",
    "- $\\Gamma$ is $A \\rightarrow (B \\rightarrow C)$\n",
    "- $\\Delta$ is empty\n",
    "- $A$ is $B$\n",
    "- $B$ is $A\\rightarrow C$\n",
    "\n",
    "Then we can use the top half of the expression to simplify it:\n",
    "$\\Gamma, A \\vdash B, \\Gamma$ is the top half of $(\\rightarrow R)$ so the top half becomes:\n",
    "$$\n",
    "A \\rightarrow (B \\rightarrow C) \\vdash A, B \\rightarrow C\n",
    "$$\n",
    "\n",
    "Applying the same rule again gives us:\n",
    "$$\n",
    "A \\rightarrow (B \\rightarrow C), B, A \\vdash C\n",
    "$$\n",
    "\n",
    "We have an implication on the left so we want to apply the $(\\rightarrow L)$ rule.\n",
    "$$\n",
    "B, A \\vdash A, C \\quad B \\rightarrow C, B, A \\vdash C\n",
    "$$\n",
    "\n",
    "The expression on the left is the imediant rule, so it is true. The expression on the right needs one final application of the $(\\rightarrow L)$ rule which produces:\n",
    "$$\n",
    "B, A \\vdash B, C \\quad C, B, A \\vdash C\n",
    "$$\n",
    "\n",
    "which are both match imediant rule so we have proved the original expression."
   ]
  }
 ],
 "metadata": {
  "kernelspec": {
   "display_name": "Python 3",
   "language": "python",
   "name": "python3"
  },
  "language_info": {
   "codemirror_mode": {
    "name": "ipython",
    "version": 3
   },
   "file_extension": ".py",
   "mimetype": "text/x-python",
   "name": "python",
   "nbconvert_exporter": "python",
   "pygments_lexer": "ipython3",
   "version": "3.5.3"
  }
 },
 "nbformat": 4,
 "nbformat_minor": 2
}
